theories/rust_typing/adequacy.v
@@ -100,7 +100,7 @@ Proof.
     iMod (na_alloc) as "(%π & Hna)".
     iDestruct ("Hfn" $! π) as (P) "[Hmain HP]".
     rewrite /initial_prog.
-    iApply (type_call_fnptr π [] [] 0 [] main main [] [] (λ _ _ _ _ _, True%I) (main_type P) [] with "[HP Hna] Hmain [] [] [] []").
+    iApply (type_call_fnptr π [] [] 0 [] main main [] [] (λ _ _ _ _ _, True%I) (main_type P) [] with "[HP ] Hmain [] [] [] [] [Hna]").
     + iIntros "_". iExists eq_refl, tt.
       iIntros (???) "#CTX #HE HL".
       iModIntro. iExists [], [], True%I.
@@ -118,6 +118,7 @@ Proof.
     + rewrite /rrust_ctx. iFrame "#".
     + by iApply big_sepL_nil.
     + by iApply big_sepL_nil.
+    + iPoseProof (na_own_acc (↑shrN) with "Hna") as "(Hna &_)"; first set_solver. iFrame.
     + iIntros (?????) "HL Hv _". done.
   - iFrame. iIntros (?? _ _ ?) "_ _ _". iApply fupd_mask_intro_discard => //. iPureIntro. by eauto.
   - iFrame.
